src/Temporal_new.v
@@ -1,0 +1,229 @@
+From Heapster Require Import
+     Permissions
+     Config
+     NoEvent
+     Typing_new.
+
+From Coq Require Import
+     Program
+     Program.Equality
+     Relations
+     Morphisms
+     Streams
+     Vector.
+
+From ExtLib Require Import
+     Structures.Functor
+     Structures.Monad.
+
+From ITree Require Import
+     ITree
+     Basics.Basics
+     Basics.MonadState
+     Basics.CategoryTheory
+     Events.Exception
+     Events.Nondeterminism
+     Events.Writer
+     Events.State
+     Events.StateFacts
+     Eq.Eq
+     Interp.Interp
+     Interp.InterpFacts.
+
+From Paco Require Import
+     paco.
+
+Import ITreeNotations.
+
+Hint Resolve no_errors_gen_mon : paco.
+Hint Resolve sbuter_gen_mon : paco.
+
+
+(** * `eq_sat_sep_sbuter` **)
+
+Definition TPred S R := CompM S R -> S -> Prop.
+Definition TPred' S R := CompM' S R -> S -> Prop.
+
+Definition eq_sat_sep_sbuter {S1 S2 R1 R2} (q:@perm (S1*S2))
+  (P1:TPred S1 R1) (P2:TPred S2 R2) :=
+  forall p Q t1 s1 t2 s2, pre q (s1,s2) -> p ⊥ q ->
+    sbuter p Q t1 s1 t2 s2 -> no_errors t2 s2 ->
+    (P1 t1 s1 <-> P2 t2 s2).
+Hint Unfold eq_sat_sep_sbuter.
+
+
+(** * `eq_sat_sep_sbuter` for state predicates **)
+
+Definition state_pred {S} R P : TPred S R := fun '_ s => P s.
+
+Definition q_similar {S1 S2} q (P1 : S1 -> Prop) (P2 : S2 -> Prop): Prop :=
+  forall s1 s2, pre q (s1,s2) -> (P1 s1 <-> P2 s2).
+
+Lemma eq_sat_state_preds {S1 S2 R1 R2} q (P1 : S1 -> Prop) (P2 : S2 -> Prop)
+  : q_similar q P1 P2 ->
+    eq_sat_sep_sbuter q (state_pred R1 P1) (state_pred R2 P2).
+Proof. intros; eauto. Qed.
+
+
+(** * `eq_sat_sep_sbuter` for logical connectives **)
+
+Lemma eq_sat_and {S1 S2 R1 R2} q (TP1 TP1' : TPred S1 R1) (TP2 TP2' : TPred S2 R2)
+  : eq_sat_sep_sbuter q TP1 TP2 -> eq_sat_sep_sbuter q TP1' TP2' ->
+    eq_sat_sep_sbuter q (TP1 /2\ TP1') (TP2 /2\ TP2').
+Proof.
+  intros esss esss' p Q t1 s1 t2 s2 pre_q sep sb no_errs.
+  rewrite (esss p Q t1 s1 t2 s2 pre_q sep sb no_errs).
+  rewrite (esss' p Q t1 s1 t2 s2 pre_q sep sb no_errs).
+  reflexivity.
+Qed.
+
+Lemma eq_sat_or {S1 S2 R1 R2} q (TP1 TP1' : TPred S1 R1) (TP2 TP2' : TPred S2 R2)
+  : eq_sat_sep_sbuter q TP1 TP2 -> eq_sat_sep_sbuter q TP1' TP2' ->
+    eq_sat_sep_sbuter q (TP1 \2/ TP1') (TP2 \2/ TP2').
+Proof.
+  intros esss esss' p Q t1 s1 t2 s2 pre_q sep sb no_errs.
+  rewrite (esss p Q t1 s1 t2 s2 pre_q sep sb no_errs).
+  rewrite (esss' p Q t1 s1 t2 s2 pre_q sep sb no_errs).
+  reflexivity.
+Qed.
+
+Notation "p -2> q" :=
+  (fun x0 x1 => p x0 x1 -> q x0 x1)
+  (at level 50, no associativity).
+
+Lemma eq_sat_impl {S1 S2 R1 R2} q (TP1 TP1' : TPred S1 R1) (TP2 TP2' : TPred S2 R2)
+  : eq_sat_sep_sbuter q TP1 TP2 -> eq_sat_sep_sbuter q TP1' TP2' ->
+    eq_sat_sep_sbuter q (TP1 -2> TP1') (TP2 -2> TP2').
+Proof.
+  intros esss esss' p Q t1 s1 t2 s2 pre_q sep sb no_errs.
+  rewrite (esss p Q t1 s1 t2 s2 pre_q sep sb no_errs).
+  rewrite (esss' p Q t1 s1 t2 s2 pre_q sep sb no_errs).
+  reflexivity.
+Qed.
+
+
+(** * `eq_sat_sep_sbuter` for `EU`  **)
+
+Inductive EU {S R} (P P' : TPred S R) t0 s0 : Prop :=
+| EU_here : P' t0 s0 -> EU P P' t0 s0
+| EU_step t1 s1 : P t0 s0 -> step t0 s0 t1 s1 -> EU P P' t1 s1 -> EU P P' t0 s0.
+
+Lemma eq_sat_EU {S1 S2 R1 R2} q (P1 P1' : TPred S1 R1) (P2 P2' : TPred S2 R2) :
+    eq_sat_sep_sbuter q P1 P2 -> eq_sat_sep_sbuter q P1' P2' ->
+    eq_sat_sep_sbuter q (EU P1 P1') (EU P2 P2').
+Proof.
+  intros eq_sat_Ps eq_sat_P's; split; intros.
+  - revert p t2 s2 H H0 H1 H2; dependent induction H3; intros.
+    + eapply EU_here, eq_sat_P's; eauto.
+    + punfold H2; red in X, H2; dependent induction H2.
+      * destruct x0; inv X.
+      * punfold H2; red in H2; destruct x; inv H2.
+      * eapply (IHEU p'); eauto.
+        -- respects; eapply sep_r; eauto.
+        -- pfold; red; eapply H6; eauto.
+      * destruct (stepsF_impl_stepF _ _ H8) as [?t2' [?s2' []]].
+        eapply EU_step; eauto.
+        -- eapply eq_sat_Ps; eauto.
+           pfold; red; econstructor 4; eauto.
+        -- eapply H4; eauto.
+           ++ respects; eapply sep_r; eauto.
+           ++ eapply step_no_errors; eauto.
+      * destruct (H6 _ _ X) as [?t2' [?s2' [? []]]].
+        eapply EU_step; eauto.
+        -- eapply eq_sat_Ps; eauto.
+           pfold; red; econstructor 5; eauto.
+        -- eapply (IHEU p'); pclearbot; eauto.
+           ++ respects; eapply sep_r; eauto.
+           ++ eapply step_no_errors; eauto.
+  - revert p t1 s1 H H0 H1 H2; dependent induction H3; intros.
+    + eapply EU_here, eq_sat_P's; eauto.
+    + punfold H2; red in X, H2; dependent induction H2.
+      1-2: destruct x; inv X.
+      * destruct (stepsF_impl_stepF _ _ H8) as [?t1' [?s1' []]].
+        eapply EU_step; eauto.
+        -- eapply eq_sat_Ps; eauto.
+           pfold; red; econstructor 3; eauto.
+        -- eapply H4; eauto.
+           respects; eapply sep_r; eauto.
+      * eapply (IHEU p'); eauto.
+        -- respects; eapply sep_r; eauto.
+        -- pfold; red; eapply H6; eauto.
+        -- eapply step_no_errors; eauto.
+      * destruct (H4 _ _ X) as [?t1' [?s1' [? []]]].
+        eapply EU_step; eauto.
+        -- eapply eq_sat_Ps; eauto.
+           pfold; red; econstructor 5; eauto.
+        -- eapply (IHEU p'); pclearbot; eauto.
+           ++ respects; eapply sep_r; eauto.
+           ++ eapply step_no_errors; eauto.
+Qed.
+
+
+(** * `eq_sat_sep_sbuter` for `EF`  **)
+
+Definition EF {S R} := @EU S R (fun _ _ => True).
+
+Lemma eq_sat_EF {S1 S2 R1 R2} q (P1 : TPred S1 R1) (P2 : TPred S2 R2) :
+    eq_sat_sep_sbuter q P1 P2 ->
+    eq_sat_sep_sbuter q (EF P1) (EF P2).
+Proof. eapply eq_sat_EU; easy. Qed.
+
+
+(** * `eq_sat_sep_sbuter` for `AF`  **)
+
+Definition AG_gen {S R} (P : TPred S R) (AG : TPred S R) t0 s0 :=
+  P t0 s0 /\ (forall t1 s1, step t0 s0 t1 s1 -> AG t1 s1).
+
+Definition AG {S R} P := paco2 (@AG_gen S R P) bot2.
+
+Lemma is_path_gen_mon {S R P} : monotone2 (@AG_gen S R P).
+Proof. repeat intro; induction IN; econstructor; eauto. Qed.
+Hint Resolve is_path_gen_mon : paco.
+
+Lemma eq_sat_AG {S1 S2 R1 R2} q (P1 : TPred S1 R1) (P2 : TPred S2 R2) :
+    eq_sat_sep_sbuter q P1 P2 ->
+    eq_sat_sep_sbuter q (AG P1) (AG P2).
+Proof.
+  intros eq_sat_Ps; split; intros.
+  - revert p t1 s1 t2 s2 H H0 H1 H2 H3; pcofix CIH; intros.
+    punfold H4; destruct H4; pfold; split; intros.
+    + eapply eq_sat_Ps; eauto.
+    + punfold H2; red in X, H2; dependent induction H2.
+      1-2: destruct x; inv X.
+      * destruct (stepsF_impl_stepF _ _ H6) as [?t1' [?s1' []]].
+        specialize (H9 _ _ X0); pclearbot; punfold H9; destruct H9.
+        eapply H4; eauto.
+        respects; eapply sep_r; eauto.
+      * right; eapply (CIH p'); eauto.
+        -- respects; eapply sep_r; eauto.
+        -- pfold; red; eapply H3; eauto.
+        -- eapply step_no_errors; eauto.
+        -- pfold; constructor; eauto.
+      * destruct (H4 _ _ X) as [?t1' [?s1' [? []]]].
+        right; eapply (CIH p'); eauto.
+        -- respects; eapply sep_r; eauto.
+        -- destruct H11; [|inversion b]; eauto.
+        -- eapply step_no_errors; eauto.
+        -- specialize (H9 _ _ x); pclearbot; eauto.
+  - revert p t1 s1 t2 s2 H H0 H1 H2 H3; pcofix CIH; intros.
+    punfold H4; destruct H4; pfold; split; intros.
+    + eapply eq_sat_Ps; eauto.
+    + punfold H2; red in X, H2; dependent induction H2.
+      * destruct x0; inv X.
+      * punfold H3; red in H3; destruct x; inv H3.
+      * right; eapply (CIH p'); eauto.
+        -- respects; eapply sep_r; eauto.
+        -- pfold; red; eapply H3; eauto.
+        -- pfold; constructor; eauto.
+      * destruct (stepsF_impl_stepF _ _ H6) as [?t2' [?s2' []]].
+        specialize (H9 _ _ X0); pclearbot; punfold H9; destruct H9.
+        eapply H4; eauto.
+        -- respects; eapply sep_r; eauto.
+        -- eapply step_no_errors; eauto.
+      * destruct (H3 _ _ X) as [?t2' [?s2' [? []]]].
+        right; eapply (CIH p' _ _ t2' s2'); eauto.
+        -- respects; eapply sep_r; eauto.
+        -- destruct H11; [|inversion H11]; eauto.
+        -- eapply step_no_errors; eauto.
+        -- specialize (H9 _ _ x); pclearbot; eauto.
+Qed.
